NI defs use low projections; restructure proofs
The main point of this change is to both to make the security definition
provable (while still ensuring security) and also to restructure the proofs.
The main change is to:
- move away from a statement of the theorem that uses a low-equivalence
relation directly and instead use one based on low projections.
- write a set of lemmas about taking steps to/from the low projections of
states, and use these to prove the single step theorem.
- the system-wide step function is also extended with a system-wide NOP

As side-effects:

These changes are fairly sweeping, so many of the old theorems are invalidated
The definitions of step functions in EvAugSemantics are rewritten to be
clearer/cleaner/better-separated:
- The single-node function is now (nid -> call -> state -> state -> event)
rather than (nid -> call -> trace -> trace) which makes it closer to the step
function that does not emit events
- A separate relation builds traces using the individual steps on states.

The main idea behind this change:

The heart of the problem with the previous definition and proof structure
is in the theorem about a single step of noninterference for an individual node.
An unusual aspect of this proof compared to one for a programming language is
that for a language, the single step theorem would compare two executions
(each with different values for secrets) for a single particular command that
is used in both executions, but in this case the command executed by a node
might be a secret itself. The fact that the command is a secret shows up in
the old low-equivalence definition: when the label of the node does not flow
to the observer, it relates any two nodes with the same label (but possibly
differing commands). This presents a problem in the old single-step theorem
(possibilistic_ni_1step_node) which we were attempting to do by cases on the
command in the first execution, and then by cases on whether the label of the
node that was executed in the first exectution flowsTo the observer or not.
In the flowsTo case, the node referred to by the chosen node id is the equal
in both executions. But in the not-flows-to case, we know nothing about what
the node looks like in the other execution (its contents are a secret).
So the command executed by the node could be anything, even an invalid
command that cannot take a step. So this old theorem with the old security
definitions is not true.

This PR attempts to fix this problem by using low projections in the
definition of security and a new proof structure. The low projections are
functions of type: {A: Type} -> label -> A -> A, that removes all the secrets
(above the label) from the thing of type A. Examples of things are nodes,
channels, and events. The new proof structure no longer has the
possibilistic_ni_1step_node theorem, but instead uses a new set of theorems
about steps to/from low projections over states (step_implies_lowproj_steps_leq,
low_proj_steps_implies_leq_step) in the proof for possibilistic_ni_1step
(which is about a system-wide step rather than a single-node step).
The (new) proof for the lemma possibilistic_ni_1step is complete
(aside from necessitating some obviously true lemmas about transitivity of
low-equivalences).

An intuition as to how this (should) fix rather than just move the problem is
that now the potential issue involving unobservable steps might show up in
the low_proj_steps_implies_leq_step lemma. However, when the step is a
command run by a secret node, the low-projection will: (1) only modify secret
state, and (2) only emit NOP-events (the low projection of a secret event is a
NOP). So for execution 2, we can choose the state and event that results from
a system-wide NOP because this should have equivalent behavior as the secret
step.

experimental/ni_coq/vfiles/EvAugSemantics.v
@@ -46,6 +46,8 @@ so the call is a piece of state that probably does not matter at the moment)
  and a downgrade event.
 *)
 
+Definition trace := list (state * event_l).
+
 Declare Scope aug_scope.
 Local Open Scope aug_scope.
 Notation "n '--->' msg":= (EvL (OutEv msg) n.(nlbl)) (at level 10) : aug_scope.
@@ -59,37 +61,32 @@ Definition head_st (t: trace) :=
         | (s', _)::_ => Some s'
     end.
 
-Inductive step_node_ev (id: node_id): call -> trace -> trace -> Prop :=
-    | SWriteChan (t: trace) s n han msg s' t:
-        head_st t = Some s ->
+Inductive step_node_ev (id: node_id): call -> state -> state -> event_l -> Prop :=
+    | SWriteChan s n han msg s':
         s.(nodes) .[?id] = Some n ->
         step_node id (WriteChannel han msg) s s' ->
-        step_node_ev id (WriteChannel han msg) t
-            ((s',  n ---> msg) :: t)
-    | SReadChan (t: trace) s n han chan msg s' t:
-        head_st t = Some s ->
+        step_node_ev id (WriteChannel han msg) s s' (n ---> msg)
+    | SReadChan s n han chan msg s':
         s.(nodes) .[?id] = Some n ->
         step_node id (ReadChannel han) s s' ->
         msg_is_head chan msg ->
-        step_node_ev id (ReadChannel han) t ((s', n <--- msg) :: t)
-    | SCreateChan (t: trace) s n lbl s' t:
+        step_node_ev id (ReadChannel han) s s' (n <--- msg)
+    | SCreateChan s n lbl s':
             (* It seems clear that no event is needed since nodes only observe
             * contents of channels indirectly via reads *)
-        head_st t = Some s ->
         s.(nodes) .[?id] = Some n ->
         step_node id (CreateChannel lbl) s s' ->
-        step_node_ev id (CreateChannel lbl) t ((s', n --- ) :: t)
-    | SCreateNode (t: trace) s n lbl h s' t:
+        step_node_ev id (CreateChannel lbl) s s' (n --- )
+    | SCreateNode s n lbl h s':
             (* model observation that a node is created ?? *)
-        head_st t = Some s ->
         s.(nodes) .[?id] = Some n ->
         step_node id (CreateNode lbl h) s s' ->
-        step_node_ev id (CreateNode lbl h) t ((s', n ---) :: t)
-    | SInternal (t: trace) s n s' t:
-        head_st t = Some s ->
+        step_node_ev id (CreateNode lbl h) s s' (n ---)
+    | SInternal s n s':
         s.(nodes) .[?id] = Some n ->
         step_node id Internal s s' ->
-        step_node_ev id Internal t ((s', n ---) :: t).
+        step_node_ev id Internal s s' (n ---).
+
 
 Definition trace_upd_head_state (t: trace) (s: state) :=
     match t with
@@ -104,21 +101,30 @@ Definition head_set_call t id c: trace :=
         | (s, e) :: t' => (s_set_call s id c, e) :: t'
     end.
 
-Inductive step_system_ev: trace -> trace -> Prop :=
-    | ValidStep id n c c' s t s' t':
-        head_st t  = Some s ->
-        head_st t' = Some s' ->
+Inductive step_system_ev: state -> state -> event_l -> Prop :=
+    | SytsemEvSkip s ell: step_system_ev s s (EvL NilEv ell)
+    | SystemEvStepNode id n c c' s s' e:
         s.(nodes) .[?id] = Some n ->
         n.(ncall) = c ->
-        step_node_ev id c t t' ->
-        step_system_ev t (head_set_call t' id c').
+        step_node_ev id c s s' e ->
+        let s'' := (s_set_call s' id c') in
+            (* Here c' is an arbitrary command. The next ABI call
+            that the node makes after the one executed here is an arbitrary one
+            of that node's choosing *)
+        step_system_ev s s'' e.
+
+Inductive step_system_ev_t: trace -> trace -> Prop :=
+    | StepTrace t s s' e:
+        head_st t = Some s -> 
+        step_system_ev s s' e ->
+        step_system_ev_t t ((s', e) :: t).
 
 Inductive step_system_ev_multi: trace -> trace -> Prop :=
     | multi_system_ev_refl t t':
-        step_system_ev t t' ->
+        step_system_ev_t t t' ->
         step_system_ev_multi t t'
     | multi_system_ev_tran t1 t2 t3:
-        step_system_ev t2 t3 ->
+        step_system_ev_t t2 t3 ->
         step_system_ev_multi t1 t2 ->
         step_system_ev_multi t1 t3.
 
