experimental/ni_coq/vfiles/LowEquivalences.v
@@ -1,14 +1,19 @@
 Require Import Coq.Lists.List.
+Require Import Coq.Sets.Ensembles.
 Import ListNotations.
 From OakIFC Require Import
-    RuntimeModel
+    Lattice
     Parameters
-    GenericMap.
+    GenericMap
+    Lattice
+    Events
+    RuntimeModel
+    EvAugSemantics.
 
-Local Open Scope map_scope.
-(*=============================================================================
-* Low Equivalences
-=============================================================================*)
+(* Ensembles don't have implicit type params and this line fixes that *)
+Arguments Ensembles.Empty_set{U}.
+
+(* TODO fix comments to also talk about low projections *)
 (* 
 This file defines "low equivalence relations" over various pieces of state.
 These are auxiliary definitions for defining the security condition.
@@ -22,40 +27,165 @@ able to see channels labeled "Bob", so _any_ pair of channels with this label
 are related even if their contents differ.
 *)
 
-Inductive chan_low_eq: level -> channel -> channel -> Prop :=
-    | ChEq ell ch1 ch2 (H: ch1 = ch2): chan_low_eq ell ch1 ch2
-    | ChNoFlow ell ch1 ch2
-        (* if the level is not high enough to read either channel,
-        * they both look the same to observers at this level *)
-        (Hlbl_eq: ch1.(clbl) = ch2.(clbl))  
-                (* Hlbl_eq makes the labels of channels publicly observable *)
-        (H1: ~(ch1.(clbl) <<L ell))
-        (H2: ~(ch2.(clbl) <<L ell)):
-        chan_low_eq ell ch1 ch2.
 
-Inductive node_low_eq: level -> node -> node -> Prop :=
-    | NodeEq ell n1 n2 (H: n1 = n2): node_low_eq ell n1 n2
-    | NodeNoFlow ell n1 n2
-        (Hlbl_eq: n1.(nlbl) = n2.(nlbl))
-                (* Hlbl_eq makes the labels of nodes publicly observable *)
-        (H1: ~(n1.(nlbl) <<L ell))
-        (H2: ~(n2.(nlbl) <<L ell)):
-        node_low_eq ell n1 n2.
+(*============================================================================
+* Empty Things
+*===========================================================================*)
+Definition empty_chan (l:level): channel := {|
+    clbl := l;
+    ms := [];
+|}.
 
-Definition chan_state_low_eq (ell: level)(chs1 chs2: chan_state): Prop :=
-    forall h, (match (chs1 .[?h]), (chs2 .[?h]) with
-        | None, None => True
-        | Some ch1, Some ch2 => chan_low_eq ell ch1 ch2
-        | _, _ => False
-    end).
+Definition empty_node (l: level): node := {|
+    nlbl := l;
+    read_handles := Empty_set;
+    write_handles := Empty_set;
+    ncall := Internal; 
+|}.
 
-Definition node_state_low_eq (ell: level)(ns1 ns2: node_state): Prop :=
-    forall h, (match (ns1 .[?h]), (ns2 .[?h]) with
-        | None, None => True
-        | Some n1, Some n2 => node_low_eq ell n1 n2
-        | _, _ => False
-    end).
+Definition empty_event (l: level): event_l := {|
+    elbl := l;
+    e := NilEv;
+|}.
+    
 
-Definition state_low_eq (ell: level)(s1 s2: state): Prop :=
-    (node_state_low_eq ell s1.(nodes) s2.(nodes)) /\
-        (chan_state_low_eq ell s1.(chans) s2.(chans)).
+(*============================================================================
+* Low Projections
+*===========================================================================*)
+
+Definition low_proj (A: Type): Type := level -> A -> A.
+
+Definition chan_low_proj (ell: level)(c: channel): channel :=
+    if(c.(clbl) <<? ell) then c else (empty_chan c.(clbl)).
+
+Definition node_low_proj (ell: level)(n: node): node :=
+    if(n.(nlbl) <<? ell) then n else (empty_node n.(nlbl)).
+
+Definition event_low_proj (ell: level)(e: event_l): event_l :=
+    if(e.(elbl) <<? ell) then e else (empty_event e.(elbl)).
+
+Definition node_state_low_proj (ell: level)(ns: node_state): node_state :=
+    fun id => match (ns id) with
+        | None => None
+        | Some n => Some (node_low_proj ell n)
+    end.
+
+Definition chan_state_low_proj (ell: level)(cs: chan_state): chan_state :=
+    fun h => match (cs h) with
+        | None => None
+        | Some c => Some (chan_low_proj ell c)
+    end.
+
+Definition state_low_proj (ell: level)(s: state): state := {|
+    nodes := node_state_low_proj ell s.(nodes);
+    chans := chan_state_low_proj ell s.(chans);
+|}.
+
+(*============================================================================
+* Low Equivalences
+*===========================================================================*)
+
+Definition low_eq {A: Type} (p: (low_proj A)):=
+    fun ell a1 a2 => (p ell a1) = (p ell a2).
+
+Definition chan_low_eq := low_eq chan_low_proj.
+Definition node_low_eq := low_eq node_low_proj.
+Definition event_low_eq := low_eq event_low_proj.
+Definition node_state_low_eq := low_eq node_state_low_proj.
+Definition chan_state_low_eq := low_eq chan_state_low_proj.
+Definition state_low_eq := low_eq state_low_proj.
+
+(*============================================================================
+* Trace Low Equivalences
+*===========================================================================*)
+
+(* We might need two different definitions of trace low-equivalence
+* depending on the top-level security condition *)
+
+(* This is a straightforward definition of trace low-equivalence
+    Roughly, it says that 
+    t1 =L t2 <-> forall i, t1[i] =L t2[i].
+
+    This definition would be useful for a 
+    "possibilistic security condition". A possibilistic security condition
+    says that two executions look the same from the perspective of an observer
+    if all _possible behaviors_ look the same if they begin from initial states
+    that look the same to the observer.
+
+    Possibilistic security conditions say that
+    forall s1 s2 t1, 
+        (s1 =L s2 -> <c, s1> => t1),
+        exists t2, <c, s2> => t2 /\ t1 =L t2.
+
+    In other words there is some way to reach an execution trace
+    that looks the same beginning from the other state.
+    
+    Trapeze uses a possibilistic definition of security:
+    https://pdfs.semanticscholar.org/809b/f2702a765b9e7dba4624a1dbc53af11579db.pdf
+    See also:
+    https://www.cs.cornell.edu/andru/papers/csfw03.pdf
+
+    and discussion in PossibilisticNI.v
+*)
+
+Inductive trace_low_eq: level -> trace -> trace -> Prop :=
+    | NilEQ ell: trace_low_eq ell [] []
+    | AddBoth ell xs xe ys ye t1 t2:
+        trace_low_eq ell t1 t2 ->
+        event_low_eq ell xe ye ->
+        state_low_eq ell xs ys ->
+        trace_low_eq ell ((xs, xe)::t1) ((ys, ye)::t2).
+
+
+(* An alternative way of specifying security for
+   concurrent systems is observational determinism, which says
+   that for any two executions that begin from low-equivalent
+   initial states, the actual observed behaviors 
+   (by contrast to possibly observed behaviors)
+   _always_ look the same.
+
+    This looks like:
+    forall s1 s2 t1 t2,
+        (s1 =L s2) /\
+        (step_multi s1) => t1 /\
+        (step_multi s2) => t2 ->
+            t1 =L t2.
+
+    If we write this top-level theorem using the straightforward
+    definition of trace low-equivalence from above, the security condition
+    would rule out *some* timing channels that we know our system does not
+    prevent (so the security condition would not work). 
+
+    The straightforward security condition would rule out the case where:
+    - The observer is L
+    - There is label L' s.t. not (L' flowsTo L)
+    - A node called Other with Label L' takes more state transitions in one execution to
+    perform some computation than in the other.
+
+    While the "Other" node is executing, it can only affect parts of the system
+    labeled L' (or higher), so for this part of a single execution, it will
+    look like a sequence where ... si =L si+1 =L si+2 ... . In other words, the
+    sub-sequence is low-equivalent. If the observer really can't measure time,
+    two sequences that differ just in the number of transitions by "Other"
+    really do look the same.
+
+    This definition of trace low-equivalence rules this out by collapsing
+    adjacent low-equivalent states (called "high stutter") in the traces.
+*)
+Inductive stut_trace_low_eq: level -> trace -> trace -> Prop :=
+    | SNilEQ ell: stut_trace_low_eq ell [] []
+    | SAddBoth ell xs xe ys ye t1 t2:
+        stut_trace_low_eq ell t1 t2 ->
+        event_low_eq ell xe ye ->
+        state_low_eq ell xs ys ->
+        stut_trace_low_eq ell ((xs, xe)::t1) ((ys, ye)::t2)
+    | SAddEqR ell xs xe ys ye t1 t2:
+        stut_trace_low_eq ell t1 ((ys, ye)::t2) ->
+        event_low_eq ell xe ye ->
+        state_low_eq ell xs ys ->
+        stut_trace_low_eq ell t1 ((xs, xe)::(ys, ye)::t2)
+    | SAddEqL ell xs xe ys ye t1 t2:
+        stut_trace_low_eq ell ((ys, ye)::t1) t2 ->
+        event_low_eq ell xe ye ->
+        state_low_eq ell xs ys ->
+        stut_trace_low_eq ell ((xs, xe)::t1) ((ys, ye)::t2).
