experimental/ni_coq/vfiles/PossibilisticNI.v
@@ -73,107 +73,82 @@ Definition conjecture_possibilistic_ni := forall ell t1_init t2_init t1n,
         (step_system_ev_multi t2_init t2n) /\
         (trace_low_eq ell t1n t2n)).
 
-Theorem possibilistic_ni_1step_node: forall ell id t1 t2 s1 s2 n1 n2 t1',
-    (head_st t1 = Some s1) ->
-    (head_st t2 = Some s2) ->
-    (s1.(nodes) .[?id] = Some n1) ->
-    (s2.(nodes) .[?id] = Some n2) ->
-    (trace_low_eq ell t1 t2) ->
-    (step_node_ev id (ncall n1) t1 t1') ->
-    (exists t2',
-        (step_node_ev id (ncall n2) t2 t2') /\
-        (trace_low_eq ell t1' t2')).
-Proof.
-    intros.
-    assert (Hsleq_s1s2: state_low_eq ell s1 s2) by
-        (eapply trace_leq_imples_head_st_leq; eassumption).
-    inversion H4; subst.
-    - (* WriteChannel *)
-        inversion H8. assert (s = s1) by congruence.
-        assert (n0 = n) by congruence. subst.
-        assert (n = n1) by congruence. subst.
-        destruct (ord_dec (nlbl n1) (ell)) eqn:Hflows.
-        + (* flows *)
-        assert (n1=n2) by
-            (eapply state_leq_and_flowsto_to_node_eq; eassumption).
-        rename n2 into n. subst.
-        (* todo need to uncons the right channel from s2 and use it
-        here instead of ch'*)
 
-        rename ch into ch1. rename ch' into ch1'.
-        specialize (other_chan_exists_from_chans_leq ell s1 s2 han ch1) as [ch2 [Hch2 Hchanleq]].
-            apply Hsleq_s1s2. assumption.
-        (*
-            note that the channels could be different because we have
-            nlbl n <<L ell  and    nlbl n <<L clbl ch1    and   nlbl n <<L clbl ch2
-            but these do not imply that clbl ch1 <<L clbl ch2 or vice versa 
-        *)
-        remember (chan_append ch2 msg) as ch2'.
-        remember (state_upd_chan han ch2'
-            (state_upd_node id n' s2)) as s2'.
-        exists ((s2', n ---> msg) :: t2). split.
-        --  (* the step happens *)
-            assert ((ncall n) = WriteChannel han msg) by congruence.
-            rewrite H9.
-            eapply SWriteChan; auto; try eassumption; try congruence.
-            rewrite Heqs2'. (* replace n' with (node_del_rhans (rhs msg) n ) in *. *)
-            rewrite Heqch2'.
-            eapply RuntimeModel.SWriteChan; auto; try eassumption; try congruence.
-            inversion Hchanleq; subst; congruence.
-        -- (* the traces are low-equivalent*)
-            constructor; try congruence.
-            constructor. reflexivity. constructor. rewrite Heqs2'.
-            * (* node_state_leq *) 
-                eapply state_upd_chan_preserves_node_state_leq.
-                eapply leq_node_updates_preserve_node_state_leq; try congruence.
-                apply Hsleq_s1s2. eapply node_low_eq_reflexive.
-            * (* chan_state_leq *)
-                rewrite Heqs2'. 
-                eapply leq_chan_updates_preserve_chan_state_leq.
-                eapply state_upd_node_preserves_chan_state_leq. apply Hsleq_s1s2.
-                assert (ch1' = chan_append ch1 msg) by
-                    (destruct (chan_append ch1 msg ); reflexivity).
-                rewrite H9, Heqch2'.
-                eapply chan_append_unwind.
-                    (* chan_low_eq ell ch1 ch2 *) (* TODO make theorem*)
-                inversion Hsleq_s1s2. specialize (H16 han).
-                    rewrite H13 in H16. rewrite Hch2 in H16. assumption.
-        + (* NOT flows *)
-Admitted. (* WIP *)
- 
-Theorem possibilistic_ni_1step: forall ell t1 t2 t1',
-    (trace_low_eq ell t1 t2) ->
-    (step_system_ev t1 t1') ->
-    (exists t2',
-        (step_system_ev t2 t2') /\
-        (trace_low_eq ell t1' t2')).
+Theorem n_low_proj_label_preserving: forall ell n,
+    (node_low_proj ell n).(nlbl) = n.(nlbl).
 Proof.
-    intros.
-    inversion H0; subst.
-    rename t' into t1_sn. rename s into s1. rename s' into s1'. rename n into n1.
-    specialize (trace_loweq_to_deref_node ell t1 t2 id s1 n1
-        H H1 H3) as [s2 [n2 [Ht2s2 Hs2n2]]].
-    specialize (possibilistic_ni_1step_node ell id
-        t1 t2 s1 s2 n1 n2 t1_sn  H1 Ht2s2 H3 Hs2n2 H H5)
-            as [t2_sn [Hnstep2 Hnstep_leq]].
-    assert (Hs2': exists s2', head_st t2_sn = Some s2'). {
-        (* this assertion is essentially re-stating node_no_steps_to_empty
-        in a way that gives us a particular head state of t2_sn *)
-        destruct t2_sn; subst.
-        - exfalso. apply (node_no_steps_to_empty t2 id (ncall n2)). assumption.
-        - exists (fst p). simpl. destruct p. reflexivity.
-    }
-    destruct Hs2' as [s2' Hs2']. 
-    remember (head_set_call t2_sn id c') as t2'.
-    exists t2'. split.
-    +  (* can step from t2_sn to t2' *)
-        subst. apply (ValidStep id n2 (ncall n2) c' s2 t2 s2' t2_sn);
-            (assumption || reflexivity).
-    + (* low-equiv t1' t2' *)
-        remember (head_set_call t1_sn id c') as t1' eqn:Ht1'.
-        apply (call_havoc_unwind ell id c' t1_sn t2_sn t1' t2');
-            (assumption || reflexivity).
-Qed. 
+Admitted.
+
+Theorem state_low_eq_from_substates: forall ell s1 s2,
+    (node_state_low_eq ell s1.(nodes) s2.(nodes)) ->
+    (chan_state_low_eq ell s1.(chans) s2.(chans)) ->
+    (state_low_eq ell s1 s2).
+Proof.
+Admitted. (* WIP *)
+
+Theorem eq_nodes_have_eq_lbls: forall n1 n2,
+    n1 = n2 -> (nlbl n1) = (nlbl n2).
+Proof. congruence. Qed.
+ 
+Theorem node_leq_imples_eq_lbls: forall ell n1 n2,
+    (node_low_eq ell n1 n2) -> (n1.(nlbl) = n2.(nlbl)).
+Proof.
+    inversion 1. unfold node_low_proj in H1.
+     destruct (n1.(nlbl) <<? ell); destruct (n2.(nlbl) <<? ell).
+    - congruence.
+    - inversion H1. reflexivity.
+    - apply eq_nodes_have_eq_lbls in H1. simpl in H1. congruence.
+    - inversion H1. congruence.
+Qed.
+
+Theorem step_implies_lowproj_steps_leq: forall ell s1 s1' e1,
+    (step_system_ev s1 s1' e1) ->
+    (exists s2' e2,
+        (step_system_ev (state_low_proj ell s1) s2' e2) /\
+        (state_low_eq ell s1' s2') /\
+        (event_low_eq ell e1 e2)).
+Proof.
+Admitted.
+
+Theorem low_proj_steps_implies_leq_step: forall ell s s1' e1,
+    (step_system_ev (state_low_proj ell s) s1' e1) ->
+    (exists s2' e2,
+        (step_system_ev s s2' e2) /\
+        (state_low_eq ell s1' s2') /\
+        (event_low_eq ell e1 e2)).
+Proof.
+Admitted.
+
+Theorem possibilistic_ni_1step: forall ell s1 s2 s1' e1,
+    (state_low_eq ell s1 s2) ->
+    (step_system_ev s1 s1' e1) ->
+    (exists s2' e2,
+        (step_system_ev s2 s2' e2) /\
+        (state_low_eq ell s1' s2') /\
+        (event_low_eq ell e1 e2)).
+Proof.
+    intros ell s1 s2 s1' e1 H_leq_s1_s2 Hstep_s1_s1'.
+    specialize (step_implies_lowproj_steps_leq ell s1 s1' e1 Hstep_s1_s1')
+        as [s3' [ e3 [Hstep_s1_s3 [H_leq_s1'_s3' H_leq_e1_e3]]]].
+    assert (H_s2_proj_s3': (step_system_ev (state_low_proj ell s2) s3' e3)).
+        { replace (state_low_proj ell s1) with 
+            (state_low_proj ell s2) in Hstep_s1_s3. assumption. }
+    specialize (low_proj_steps_implies_leq_step ell s2 s3' e3 H_s2_proj_s3')
+        as [s2' [ e2 [Hstep_s2_s2' [H_leq_s3'_s2' H_leq_e3_e2]]]].
+    exists s2', e2. split. assumption. split.
+    - admit. (* transitivity of state_low_eq *)
+    - admit. (* transitivity of event_low_eq *)
+Admitted.
+
+Theorem possibilistic_ni_unwind_t: forall ell t1 t2 t1',
+(trace_low_eq ell t1 t2) ->
+(step_system_ev_t t1 t1') ->
+(exists t2',
+    (step_system_ev_t t2 t2') /\
+    (trace_low_eq ell t1' t2')).
+Proof.
+    (* Should make use of possibilistic_ni_1step *)
+Admitted. (* WIP *)
 
 Theorem possibilistic_ni: conjecture_possibilistic_ni.
 Proof.
@@ -185,7 +160,7 @@ induction t1n.
         exfalso. apply (no_steps_to_empty t1_init Ht1_mstep_t1n).
     - (* inductive case *)
     inversion Ht1_mstep_t1n ; subst.
-        + specialize (possibilistic_ni_1step ell t1_init t2_init
+        + specialize (possibilistic_ni_unwind_t ell t1_init t2_init
             (a::t1n) Hinit_tleq H) as [t2n [E1 E2]].
             exists t2n. split. constructor. assumption. assumption.
         + rename Ht1_mstep_t1n into Ht1_mstep_at1n.
@@ -196,7 +171,7 @@ induction t1n.
           specialize (IHt1n ltac:(assumption))
             as [t2n [Hm_t2_init_t2n Hleq_t1n_t2n]].
         specialize (step_system_multi_extends _ (a::t1n) ltac:(eauto)) as E2.
-        specialize (possibilistic_ni_1step ell t1n t2n (a::t1n) Hleq_t1n_t2n E2)
+        specialize (possibilistic_ni_unwind_t ell t1n t2n (a::t1n) Hleq_t1n_t2n E2)
             as [t2n' [Hs_t2n_t2n' Hleq_at1n_t2n']].
         exists t2n'. split.
         apply (step_system_transitive t2_init t2n t2n'). assumption.
